simple while language including parsing

ReadFileNative.cs
@@ -1,0 +1,14 @@
+using System;
+using System.IO;
+
+public partial class @FileSystem {
+
+    public static void ReadCmdLine(out char[] result) {
+        String[] arguments = Environment.GetCommandLineArgs();
+        if (arguments.Length <= 1) {
+            result = Console.In.ReadToEnd().ToCharArray();
+        } else {
+            result = File.ReadAllText(arguments[1]).ToCharArray();
+        }
+    }
+}
